FxyLang/Implementation/Syntax.lean
@@ -4,12 +4,14 @@
   Authors: Arthur Paulino
 -/
 
+/- We are going to use Lean's syntax system to parse Fxy source code -/
+
 declare_syntax_cat              literal
-syntax ("-" noWs)? num        : literal
-syntax str                    : literal
-syntax "true"                 : literal
-syntax "false"                : literal
-syntax ("-" noWs)? scientific : literal
+syntax ("-" noWs)? num        : literal -- int
+syntax str                    : literal -- str
+syntax "true"                 : literal -- bool (false)
+syntax "false"                : literal -- bool (true)
+syntax ("-" noWs)? scientific : literal -- float
 
 declare_syntax_cat binop
 syntax " + "     : binop
@@ -21,21 +23,23 @@ syntax " <= "    : binop
 syntax " > "     : binop
 syntax " >= "    : binop
 
-declare_syntax_cat                            expression
-syntax literal                              : expression -- literal
-syntax withPosition(
-  "[ " colGt literal,* " ]")                : expression -- list
-syntax:51 ident                             : expression -- variable
-syntax:49 expression (colGt expression:50)+ : expression -- application
-syntax:48 " ! " expression                  : expression -- the only unary op
-syntax:48 expression binop expression       : expression -- binary operator
-syntax " ( " expression " ) "               : expression
+declare_syntax_cat                               expression
+syntax literal                                 : expression -- literal
+syntax withPosition("[ " colGt literal,* " ]") : expression -- list
+syntax:51 ident                                : expression -- variable
+
+/-- application. The `+` means that we're expecting at least one element -/
+syntax:49 expression (colGt expression:50)+ : expression
+
+syntax:48 " ! " expression            : expression -- the only unary op
+syntax:48 expression binop expression : expression -- binary operator
+syntax " ( " expression " ) "         : expression
 
 declare_syntax_cat                      program
 declare_syntax_cat                      programSeq
 syntax withPosition((colGe program)+) : programSeq -- seq
 
-syntax "skip"                                       : program
+syntax "skip"                                       : program -- skip
 syntax withPosition(ident+ colGt " := " programSeq) : program -- decl
 syntax expression                                   : program -- eval
 syntax withPosition(
